unverified/reg_alloc/reg_alloc.sml
@@ -1,18 +1,18 @@
 structure reg_alloc = struct
-  type unit =  unit;
+  type unit = unit
   datatype reg_alloc_tag =  Stemp
-                         |  Atemp
-                         |  Fixed of  int;
+  |  Atemp
+  |  Fixed of  int;
   datatype 'a sptree_spt =  Bs of  'a sptree_spt *  'a  *  'a sptree_spt
-                         |  Bn of  'a sptree_spt *  'a sptree_spt
-                         |  Ls of  'a
-                          |  Ln;
+  |  Bn of  'a sptree_spt *  'a sptree_spt
+  |  Ls of  'a
+   |  Ln;
   datatype reg_alloc_clash_tree =  Seq of  reg_alloc_clash_tree *  reg_alloc_clash_tree
-                                |  Branch of  unit sptree_spt option *  reg_alloc_clash_tree *  reg_alloc_clash_tree
-                                |  Set of  unit sptree_spt
-                                |  Delta of  int list *  int list;
-  exception  Writeerror of  unit;
-  exception  Readerror of  unit;
+  |  Branch of  unit sptree_spt option *  reg_alloc_clash_tree *  reg_alloc_clash_tree
+  |  Set of  unit sptree_spt
+  |  Delta of  int list *  int list;
+  datatype reg_alloc_algorithm =  Irc
+  |  Simple;
   exception  Fail of  char list;
   fun  even v1 =
     if  (v1 = 0)
@@ -29,147 +29,10 @@ structure reg_alloc = struct
      |   v2::v1 =>  (v3 v2::(map v3 v1));
   fun  fst v3 =  case  v3 of  (v2,v1) =>  v2;
   fun  snd v3 =  case  v3 of  (v2,v1) =>  v1;
-  fun  lookup v7 v8 =
-    case  v8
-    of  Ln =>  NONE
-    |   Ls(v1) =>  (if  (v7 = 0)
-                    then  (SOME(v1))
-                    else  NONE)
-    |   Bn(v3,v2) =>  (if  (v7 = 0)
-                       then  NONE
-                        else  (lookup ((let val  k = v7 - 1
-                                         in
-                                          if  (k < 0)
-                                          then  0
-                                           else  k
-                                         end) div 2) (if  (even v7)
-                                                      then  v3
-                                                       else  v2)))
-    |   Bs(v6,v5,v4) =>  (if  (v7 = 0)
-                          then  (SOME(v5))
-                          else  (lookup ((let val  k = v7 - 1
-                                           in
-                                            if  (k < 0)
-                                            then  0
-                                             else  k
-                                           end) div 2) (if  (even v7)
-                                                        then  v6
-                                                         else  v4)));
-  fun  insert v7 v8 v9 =
-    case  v9
-    of  Ln =>  (if  (v7 = 0)
-                then  (Ls(v8))
-                else  (if  (even v7)
-                       then  (Bn(insert ((let val  k = v7 - 1
-                                           in
-                                            if  (k < 0)
-                                            then  0
-                                             else  k
-                                           end) div 2) v8 Ln,Ln))
-                       else  (Bn(Ln,insert ((let val  k = v7 - 1
-                                              in
-                                               if  (k < 0)
-                                               then  0
-                                                else  k
-                                              end) div 2) v8 Ln))))
-    |   Ls(v1) =>  (if  (v7 = 0)
-                    then  (Ls(v8))
-                    else  (if  (even v7)
-                           then  (Bs(insert ((let val  k = v7 - 1
-                                               in
-                                                if  (k < 0)
-                                                then  0
-                                                 else  k
-                                               end) div 2) v8 Ln,v1,Ln))
-                           else  (Bs(Ln,v1,insert ((let val  k = v7 - 1
-                                                     in
-                                                      if  (k < 0)
-                                                      then  0
-                                                       else  k
-                                                     end) div 2) v8 Ln))))
-    |   Bn(v3,v2) =>  (if  (v7 = 0)
-                       then  (Bs(v3,v8,v2))
-                       else  (if  (even v7)
-                              then  (Bn(insert ((let val  k = v7 - 1
-                                                  in
-                                                   if  (k < 0)
-                                                   then  0
-                                                    else  k
-                                                  end) div 2) v8 v3,v2))
-                              else  (Bn(v3,insert ((let val  k = v7 - 1
-                                                     in
-                                                      if  (k < 0)
-                                                      then  0
-                                                       else  k
-                                                     end) div 2) v8 v2))))
-    |   Bs(v6,v5,v4) =>  (if  (v7 = 0)
-                          then  (Bs(v6,v8,v4))
-                          else  (if  (even v7)
-                                 then  (Bs(insert ((let val  k = v7 - 1
-                                                     in
-                                                      if  (k < 0)
-                                                      then  0
-                                                       else  k
-                                                     end) div 2) v8 v6,v5,v4))
-                                 else  (Bs(v6,v5,insert ((let val  k =
-                                                            v7 - 1
-                                                           in
-                                                            if  (k < 0)
-                                                            then  0
-                                                             else  k
-                                                           end) div 2) v8 v4))));
-  fun  lrnext v1 =
-    if  (v1 = 0)
-    then  1
-     else  (2 * (lrnext ((let val  k = v1 - 1
-                           in
-                            if  (k < 0)
-                            then  0
-                             else  k
-                           end) div 2)));
-  fun  foldi v9 v10 v12 v11 =
-    case  v11
-    of  Ln =>  v12
-    |   Ls(v1) =>  (v9 v10 v1 v12)
-    |   Bn(v4,v3) =>  (let val  v2 = lrnext v10
-                        in
-                         foldi v9 (v10 + v2) (foldi v9 (v10 + (2 * v2)) v12 v4) v3
-                        end)
-    |   Bs(v8,v7,v6) =>  (let val  v5 = lrnext v10
-                           in
-                            foldi v9 (v10 + v5) (v9 v10 v7 (foldi v9 (v10 + (2 * v5)) v12 v8)) v6
-                           end);
-  fun  toalist v4 =
-    foldi (fn  v3 => (fn  v2 => (fn  v1 => ((v3,v2)::v1)))) 0 [] v4;
-  fun  fromalist v5 =
-    case  v5
-    of  []  =>  Ln
-    |   v4::v3 =>  (case  v4
-                    of  (v2,v1) =>  (insert v2 v1 (fromalist v3)));
-  fun  map_1 v7 v8 =
-    case  v8
-    of  Ln =>  Ln
-    |   Ls(v1) =>  (Ls(v7 v1))
-    |   Bn(v3,v2) =>  (Bn(map_1 v7 v3,map_1 v7 v2))
-    |   Bs(v6,v5,v4) =>  (Bs(map_1 v7 v6,v7 v5,map_1 v7 v4));
   fun  member v4 v3 =
     case  v3
     of  []  =>  (0 < 0)
     |   v2::v1 =>  ((v4 = v2) orelse  (member v4 v1));
-  fun  append v3 v4 =
-    case  v3
-    of  []  =>  v4
-    |   v2::v1 =>  (v2::(append v1 v4));
-  fun  null v3 =
-    case  v3
-    of  []  =>  (0 <= 0)
-    |   v2::v1 =>  (0 < 0);
-  fun  filter v3 v4 =
-    case  v4
-    of  []  =>  []
-     |   v2::v1 =>  (if  (v3 v2)
-                     then  (v2::(filter v3 v1))
-                     else  (filter v3 v1));
   fun  snoc v4 v3 =
     case  v3
     of  []  =>  [v4]
@@ -188,10 +51,10 @@ structure reg_alloc = struct
                                             then  0
                                              else  k
                                            end)));
-  fun  length v3 =
+  fun  append v3 v4 =
     case  v3
-    of  []  =>  0
-    |   v2::v1 =>  ((length v1) + 1);
+    of  []  =>  v4
+    |   v2::v1 =>  (v2::(append v1 v4));
   fun  part v3 v6 v4 v5 =
     case  v6
     of  []  =>  (v4,v5)
@@ -207,27 +70,157 @@ structure reg_alloc = struct
                        case  v3
                        of  (v2,v1) =>  (append (append (qsort v7 v2) [v6]) (qsort v7 v1))
                      end);
+  fun  lookup_1 v7 v8 =
+  case  v8
+  of  Ln =>  NONE
+  |   Ls(v1) =>  (if  (v7 = 0)
+  then  (SOME(v1))
+  else  NONE)
+  |   Bn(v3,v2) =>  (if  (v7 = 0)
+  then  NONE
+   else  (lookup_1 ((let val  k = v7 - 1
+   in
+    if  (k < 0)
+  then  0
+   else  k
+   end) div 2) (if  (even v7)
+  then  v3
+   else  v2)))
+  |   Bs(v6,v5,v4) =>  (if  (v7 = 0)
+  then  (SOME(v5))
+  else  (lookup_1 ((let val  k = v7 - 1
+   in
+    if  (k < 0)
+  then  0
+   else  k
+   end) div 2) (if  (even v7)
+  then  v6
+   else  v4)));
+  fun  insert_1 v7 v8 v9 =
+  case  v9
+  of  Ln =>  (if  (v7 = 0)
+  then  (Ls(v8))
+  else  (if  (even v7)
+  then  (Bn(insert_1 ((let val  k = v7 - 1
+   in
+    if  (k < 0)
+  then  0
+   else  k
+   end) div 2) v8 Ln,Ln))
+  else  (Bn(Ln,insert_1 ((let val  k = v7 - 1
+   in
+    if  (k < 0)
+  then  0
+   else  k
+   end) div 2) v8 Ln))))
+  |   Ls(v1) =>  (if  (v7 = 0)
+  then  (Ls(v8))
+  else  (if  (even v7)
+  then  (Bs(insert_1 ((let val  k = v7 - 1
+   in
+    if  (k < 0)
+  then  0
+   else  k
+   end) div 2) v8 Ln,v1,Ln))
+  else  (Bs(Ln,v1,insert_1 ((let val  k = v7 - 1
+   in
+    if  (k < 0)
+  then  0
+   else  k
+   end) div 2) v8 Ln))))
+  |   Bn(v3,v2) =>  (if  (v7 = 0)
+  then  (Bs(v3,v8,v2))
+  else  (if  (even v7)
+  then  (Bn(insert_1 ((let val  k = v7 - 1
+   in
+    if  (k < 0)
+  then  0
+   else  k
+   end) div 2) v8 v3,v2))
+  else  (Bn(v3,insert_1 ((let val  k = v7 - 1
+   in
+    if  (k < 0)
+  then  0
+   else  k
+   end) div 2) v8 v2))))
+  |   Bs(v6,v5,v4) =>  (if  (v7 = 0)
+  then  (Bs(v6,v8,v4))
+  else  (if  (even v7)
+  then  (Bs(insert_1 ((let val  k = v7 - 1
+   in
+    if  (k < 0)
+  then  0
+   else  k
+   end) div 2) v8 v6,v5,v4))
+  else  (Bs(v6,v5,insert_1 ((let val  k = v7 - 1
+   in
+    if  (k < 0)
+  then  0
+   else  k
+   end) div 2) v8 v4))));
+  fun  lrnext v1 =
+  if  (v1 = 0)
+  then  1
+   else  (2 * (lrnext ((let val  k = v1 - 1
+   in
+    if  (k < 0)
+  then  0
+   else  k
+   end) div 2)));
+  fun  foldi v9 v10 v12 v11 =
+  case  v11
+  of  Ln =>  v12
+  |   Ls(v1) =>  (v9 v10 v1 v12)
+  |   Bn(v4,v3) =>  (let val  v2 = lrnext v10
+   in
+    foldi v9 (v10 + v2) (foldi v9 (v10 + (2 * v2)) v12 v4) v3
+   end)
+  |   Bs(v8,v7,v6) =>  (let val  v5 = lrnext v10
+   in
+    foldi v9 (v10 + v5) (v9 v10 v7 (foldi v9 (v10 + (2 * v5)) v12 v8)) v6
+   end);
+  fun  toalist v4 =
+    foldi (fn  v3 => (fn  v2 => (fn  v1 => ((v3,v2)::v1)))) 0 [] v4;
+  fun  map_1 v7 v8 =
+  case  v8
+  of  Ln =>  Ln
+  |   Ls(v1) =>  (Ls(v7 v1))
+  |   Bn(v3,v2) =>  (Bn(map_1 v7 v3,map_1 v7 v2))
+  |   Bs(v6,v5,v4) =>  (Bs(map_1 v7 v6,v7 v5,map_1 v7 v4));
+  fun  count_list_aux v2 v1 =
+  if  (v2 = 0)
+  then  v1
+   else  (count_list_aux (let val  k = v2 - 1
+   in
+    if  (k < 0)
+  then  0
+   else  k
+   end) (let val  k = v2 - 1
+   in
+    if  (k < 0)
+  then  0
+   else  k
+   end::v1));
+  fun  count_list v1 =  count_list_aux v1 [] ;
   fun  list_remap v12 v13 =
-    case  v12
-    of  []  =>  (case  v13
-                 of  (v4,v3) =>  (case  v3 of  (v2,v1) =>  (v4,(v2,v1))))
-    |   v11::v10 =>  (case  v13
-                      of  (v9,v8) =>  (case  v8
-                                       of  (v7,v6) =>  (case  (lookup v11 v9)
-                                                        of  NONE =>  (list_remap v10 (insert v11 v6 v9,(insert v6 v11 v7,v6 + 1)))
-                                                        |   (SOME(v5)) =>  (list_remap v10 (v9,(v7,v6))))));
+  case  v12
+  of  []  =>  (case  v13 of  (v4,v3) =>  (case  v3 of  (v2,v1) =>  (v4,(v2,v1))))
+  |   v11::v10 =>  (case  v13
+  of  (v9,v8) =>  (case  v8
+  of  (v7,v6) =>  (case  (lookup_1 v11 v9)
+  of  NONE =>  (list_remap v10 (insert_1 v11 v6 v9,(insert_1 v6 v11 v7,v6 + 1)))
+  |   (SOME(v5)) =>  (list_remap v10 (v9,(v7,v6))))));
   fun  mk_bij_aux v11 v12 =
-    case  v11
-    of  Delta(v2,v1) =>  (list_remap v2 (list_remap v1 v12))
-    |   Set(v3) =>  (list_remap (map fst (toalist v3)) v12)
-    |   Branch(v8,v7,v6) =>  (let val  v5 =
-                                mk_bij_aux v6 (mk_bij_aux v7 v12)
-                              in
-                                case  v8
-                                of  NONE =>  v5
-                                |   SOME(v4) =>  (list_remap (map fst (toalist v4)) v5)
-                              end)
-    |   Seq(v10,v9) =>  (mk_bij_aux v10 (mk_bij_aux v9 v12));
+  case  v11
+  of  Delta(v2,v1) =>  (list_remap v2 (list_remap v1 v12))
+  |   Set(v3) =>  (list_remap (List.map fst (toalist v3)) v12)
+  |   Branch(v8,v7,v6) =>  (let val  v5 = mk_bij_aux v6 (mk_bij_aux v7 v12)
+  in
+    case  v8
+  of  NONE =>  v5
+  |   SOME(v4) =>  (list_remap (List.map fst (toalist v4)) v5)
+  end)
+  |   Seq(v10,v9) =>  (mk_bij_aux v10 (mk_bij_aux v9 v12));
   fun  mk_bij v6 =
     let val  v5 = mk_bij_aux v6 (Ln,(Ln,0))
     in
@@ -236,759 +229,1047 @@ structure reg_alloc = struct
   fun  is_phy_var v1 =  (v1 mod 2) = 0;
   fun  sp_default v3 =
     (fn  v2 =>
-      case  (lookup v2 v3)
+      case  (lookup_1 v2 v3)
       of  NONE =>  (if  (is_phy_var v2)
-                    then  (v2 div 2)
-                    else  v2)
+      then  (v2 div 2)
+      else  v2)
       |   SOME(v1) =>  v1);
   fun  extract_tag v2 =
     case  v2
     of  Fixed(v1) =>  v1
     |   Atemp =>  0
     |   Stemp =>  0;
+  fun  fromalist v5 =
+  case  v5
+  of  []  =>  Ln
+  |   v4::v3 =>  (case  v4 of  (v2,v1) =>  (insert_1 v2 v1 (fromalist v3)));
+  fun  sort_moves v7 =
+    qsort (fn  v6 =>
+      (case  v6
+      of  (v5,v4) =>  (fn  v3 => (case  v3 of  (v2,v1) =>  (v5 > v2))))) v7;
+  fun  smerge v10 v9 =
+  case  v10
+  of  []  =>  v9
+  |   v8::v7 =>  (case  v9
+  of  []  =>  (v8::v7)
+  |   (v6::v5) =>  (case  v6
+  of  (v4,v3) =>  (case  v8
+  of  (v2,v1) =>  (if  (v2 >= v4)
+  then  ((v2,v1)::(smerge v7 ((v4,v3)::v5)))
+  else  ((v4,v3)::(smerge ((v2,v1)::v7) v5))))));
+  fun  pair_rename v11 =
+    (fn  v9 =>
+      (fn  v10 =>
+        case  (v9,v10)
+        of  (v8,v7) =>  (case  v7
+        of  (v6,v5) =>  (case  v5
+        of  (v4,v3) =>  (let val  v2 =
+          if  (v4 = v8)
+          then  v11
+           else  v4
+            val  v1 =
+          if  (v3 = v8)
+          then  v11
+           else  v3
+         in
+          (v6,(v2,v1))
+        end)))));
+  fun  safe_div v2 =
+    (fn  v1 =>
+      if  (v1 = 0)
+      then  0
+       else  (v2 div v1));
+  fun  lookup_any v4 =
+    (fn  v3 =>
+      (fn  v2 =>
+        case  (lookup_1 v4 v3)
+        of  NONE =>  v2
+        |   SOME(v1) =>  v1));
   fun  tag_col v2 =
     case  v2
     of  Fixed(v1) =>  v1
     |   Atemp =>  0
     |   Stemp =>  0;
   fun  unbound_colour v3 v4 =
-    case  v4
-    of  []  =>  v3
-    |   v2::v1 =>  (if  (v3 < v2)
-                    then  v3
-                     else  (if  (v2 = v3)
-                            then  (unbound_colour (v3 + 1) v1)
-                            else  (unbound_colour v3 v1)));
+  case  v4
+  of  []  =>  v3
+  |   v2::v1 =>  (if  (v3 < v2)
+  then  v3
+   else  (if  (v2 = v3)
+  then  (unbound_colour (v3 + 1) v1)
+  else  (unbound_colour v3 v1)));
   fun  pri_move_insert v3 =
     (fn  v4 =>
       (fn  v5 =>
         (fn  v2 =>
-          case  (lookup v4 v2)
-          of  NONE =>  (insert v4 [(v3,v5)] v2)
-          |   SOME(v1) =>  (insert v4 ((v3,v5)::v1) v2))));
+          case  (lookup_1 v4 v2)
+          of  NONE =>  (insert_1 v4 [(v3,v5)] v2)
+          |   SOME(v1) =>  (insert_1 v4 ((v3,v5)::v1) v2))));
   fun  undir_move_insert v2 =
     (fn  v3 =>
       (fn  v4 =>
-        (fn  v1 =>
-          pri_move_insert v2 v3 v4 (pri_move_insert v2 v4 v3 v1))));
+        (fn  v1 => pri_move_insert v2 v3 v4 (pri_move_insert v2 v4 v3 v1))));
   fun  moves_to_sp v9 v8 =
-    case  v9
-    of  []  =>  v8
-    |   v7::v6 =>  (let val  v5 = v7
-                     in
-                      case  v5
-                      of  (v4,v3) =>  (case  v3
-                                       of  (v2,v1) =>  (moves_to_sp v6 (undir_move_insert v4 v2 v1 v8)))
-                    end);
+  case  v9
+  of  []  =>  v8
+  |   v7::v6 =>  (let val  v5 = v7
+   in
+    case  v5
+  of  (v4,v3) =>  (case  v3
+  of  (v2,v1) =>  (moves_to_sp v6 (undir_move_insert v4 v2 v1 v8)))
+  end);
   fun  resort_moves v8 =
     map_1 (fn  v7 =>
-            (map snd (qsort (fn  v6 =>
-                              (case  v6
-                               of  (v5,v4) =>  (fn  v3 =>
-                                                (case  v3
-                                                 of  (v2,v1) =>  (v5 > v2))))) v7))) v8;
-  datatype reg_alloc_ira_state =  Recordtypeira_state of  (int *  int list) *  (int *  reg_alloc_tag) *  (int *  int) *  int *  int list *  int list *  int list;
-  fun  ira_state_adj_ls v8 =
-    case  v8 of  Recordtypeira_state(v7,v6,v5,v4,v3,v2,v1) =>  v7;
-  fun  ira_state_node_tag v8 =
-    case  v8 of  Recordtypeira_state(v7,v6,v5,v4,v3,v2,v1) =>  v6;
-  fun  ira_state_degrees v8 =
-    case  v8 of  Recordtypeira_state(v7,v6,v5,v4,v3,v2,v1) =>  v5;
-  fun  ira_state_dim v8 =
-    case  v8 of  Recordtypeira_state(v7,v6,v5,v4,v3,v2,v1) =>  v4;
-  fun  ira_state_simp_wl v8 =
-    case  v8 of  Recordtypeira_state(v7,v6,v5,v4,v3,v2,v1) =>  v3;
-  fun  ira_state_spill_wl v8 =
-    case  v8 of  Recordtypeira_state(v7,v6,v5,v4,v3,v2,v1) =>  v2;
-  fun  ira_state_stack v8 =
-    case  v8 of  Recordtypeira_state(v7,v6,v5,v4,v3,v2,v1) =>  v1;
-  fun  ira_state_adj_ls_fupd v8 =
-    (fn  v9 =>
-      case  v9
-      of  Recordtypeira_state(v7,v6,v5,v4,v3,v2,v1) =>  (Recordtypeira_state(v8 v7,v6,v5,v4,v3,v2,v1)));
-  fun  ira_state_node_tag_fupd v8 =
-    (fn  v9 =>
-      case  v9
-      of  Recordtypeira_state(v7,v6,v5,v4,v3,v2,v1) =>  (Recordtypeira_state(v7,v8 v6,v5,v4,v3,v2,v1)));
-  fun  ira_state_degrees_fupd v8 =
-    (fn  v9 =>
-      case  v9
-      of  Recordtypeira_state(v7,v6,v5,v4,v3,v2,v1) =>  (Recordtypeira_state(v7,v6,v8 v5,v4,v3,v2,v1)));
-  fun  ira_state_dim_fupd v8 =
-    (fn  v9 =>
-      case  v9
-      of  Recordtypeira_state(v7,v6,v5,v4,v3,v2,v1) =>  (Recordtypeira_state(v7,v6,v5,v8 v4,v3,v2,v1)));
-  fun  ira_state_simp_wl_fupd v8 =
-    (fn  v9 =>
-      case  v9
-      of  Recordtypeira_state(v7,v6,v5,v4,v3,v2,v1) =>  (Recordtypeira_state(v7,v6,v5,v4,v8 v3,v2,v1)));
-  fun  ira_state_spill_wl_fupd v8 =
-    (fn  v9 =>
-      case  v9
-      of  Recordtypeira_state(v7,v6,v5,v4,v3,v2,v1) =>  (Recordtypeira_state(v7,v6,v5,v4,v3,v8 v2,v1)));
-  fun  ira_state_stack_fupd v8 =
-    (fn  v9 =>
-      case  v9
-      of  Recordtypeira_state(v7,v6,v5,v4,v3,v2,v1) =>  (Recordtypeira_state(v7,v6,v5,v4,v3,v2,v8 v1)));
-  datatype reg_alloc_ra_state =  Recordtypera_state of  int list list *  reg_alloc_tag list *  int list *  int *  int list *  int list *  int list;
-  fun  ra_state_adj_ls v8 =
-    case  v8 of  Recordtypera_state(v7,v6,v5,v4,v3,v2,v1) =>  v7;
-  fun  ra_state_node_tag v8 =
-    case  v8 of  Recordtypera_state(v7,v6,v5,v4,v3,v2,v1) =>  v6;
-  fun  ra_state_degrees v8 =
-    case  v8 of  Recordtypera_state(v7,v6,v5,v4,v3,v2,v1) =>  v5;
-  fun  ra_state_dim v8 =
-    case  v8 of  Recordtypera_state(v7,v6,v5,v4,v3,v2,v1) =>  v4;
-  fun  ra_state_simp_wl v8 =
-    case  v8 of  Recordtypera_state(v7,v6,v5,v4,v3,v2,v1) =>  v3;
-  fun  ra_state_spill_wl v8 =
-    case  v8 of  Recordtypera_state(v7,v6,v5,v4,v3,v2,v1) =>  v2;
-  fun  ra_state_stack v8 =
-    case  v8 of  Recordtypera_state(v7,v6,v5,v4,v3,v2,v1) =>  v1;
-  fun  ra_state_adj_ls_fupd v8 =
-    (fn  v9 =>
-      case  v9
-      of  Recordtypera_state(v7,v6,v5,v4,v3,v2,v1) =>  (Recordtypera_state(v8 v7,v6,v5,v4,v3,v2,v1)));
-  fun  ra_state_node_tag_fupd v8 =
-    (fn  v9 =>
-      case  v9
-      of  Recordtypera_state(v7,v6,v5,v4,v3,v2,v1) =>  (Recordtypera_state(v7,v8 v6,v5,v4,v3,v2,v1)));
-  fun  ra_state_degrees_fupd v8 =
-    (fn  v9 =>
-      case  v9
-      of  Recordtypera_state(v7,v6,v5,v4,v3,v2,v1) =>  (Recordtypera_state(v7,v6,v8 v5,v4,v3,v2,v1)));
-  fun  ra_state_dim_fupd v8 =
-    (fn  v9 =>
-      case  v9
-      of  Recordtypera_state(v7,v6,v5,v4,v3,v2,v1) =>  (Recordtypera_state(v7,v6,v5,v8 v4,v3,v2,v1)));
-  fun  ra_state_simp_wl_fupd v8 =
-    (fn  v9 =>
-      case  v9
-      of  Recordtypera_state(v7,v6,v5,v4,v3,v2,v1) =>  (Recordtypera_state(v7,v6,v5,v4,v8 v3,v2,v1)));
-  fun  ra_state_spill_wl_fupd v8 =
-    (fn  v9 =>
-      case  v9
-      of  Recordtypera_state(v7,v6,v5,v4,v3,v2,v1) =>  (Recordtypera_state(v7,v6,v5,v4,v3,v8 v2,v1)));
-  fun  ra_state_stack_fupd v8 =
-    (fn  v9 =>
-      case  v9
-      of  Recordtypera_state(v7,v6,v5,v4,v3,v2,v1) =>  (Recordtypera_state(v7,v6,v5,v4,v3,v2,v8 v1)));
+      (List.map snd (qsort (fn  v6 =>
+        (case  v6
+        of  (v5,v4) =>  (fn  v3 => (case  v3 of  (v2,v1) =>  (v5 > v2))))) v7))) v8;
+  datatype reg_alloc_ira_state =  Recordtypeira_state of  (int *  int list) *  (int *  reg_alloc_tag) *  (int *  int) *  int *  int list *  int list *  int list *  (int *  (int *  int)) list *  (int *  (int *  int)) list *  (int *  int option) *  (int *  bool) *  int list;
+  fun  ira_state_adj_ls v13 =
+    case  v13
+    of  Recordtypeira_state(v12,v11,v10,v9,v8,v7,v6,v5,v4,v3,v2,v1) =>  v12;
+  fun  ira_state_node_tag v13 =
+    case  v13
+    of  Recordtypeira_state(v12,v11,v10,v9,v8,v7,v6,v5,v4,v3,v2,v1) =>  v11;
+  fun  ira_state_degrees v13 =
+    case  v13
+    of  Recordtypeira_state(v12,v11,v10,v9,v8,v7,v6,v5,v4,v3,v2,v1) =>  v10;
+  fun  ira_state_dim v13 =
+    case  v13
+    of  Recordtypeira_state(v12,v11,v10,v9,v8,v7,v6,v5,v4,v3,v2,v1) =>  v9;
+  fun  ira_state_simp_wl v13 =
+    case  v13
+    of  Recordtypeira_state(v12,v11,v10,v9,v8,v7,v6,v5,v4,v3,v2,v1) =>  v8;
+  fun  ira_state_spill_wl v13 =
+    case  v13
+    of  Recordtypeira_state(v12,v11,v10,v9,v8,v7,v6,v5,v4,v3,v2,v1) =>  v7;
+  fun  ira_state_freeze_wl v13 =
+    case  v13
+    of  Recordtypeira_state(v12,v11,v10,v9,v8,v7,v6,v5,v4,v3,v2,v1) =>  v6;
+  fun  ira_state_avail_moves_wl v13 =
+    case  v13
+    of  Recordtypeira_state(v12,v11,v10,v9,v8,v7,v6,v5,v4,v3,v2,v1) =>  v5;
+  fun  ira_state_unavail_moves_wl v13 =
+    case  v13
+    of  Recordtypeira_state(v12,v11,v10,v9,v8,v7,v6,v5,v4,v3,v2,v1) =>  v4;
+  fun  ira_state_coalesced v13 =
+    case  v13
+    of  Recordtypeira_state(v12,v11,v10,v9,v8,v7,v6,v5,v4,v3,v2,v1) =>  v3;
+  fun  ira_state_move_related v13 =
+    case  v13
+    of  Recordtypeira_state(v12,v11,v10,v9,v8,v7,v6,v5,v4,v3,v2,v1) =>  v2;
+  fun  ira_state_stack v13 =
+    case  v13
+    of  Recordtypeira_state(v12,v11,v10,v9,v8,v7,v6,v5,v4,v3,v2,v1) =>  v1;
+  fun  ira_state_adj_ls_fupd v13 =
+    (fn  v14 =>
+      case  v14
+      of  Recordtypeira_state(v12,v11,v10,v9,v8,v7,v6,v5,v4,v3,v2,v1) =>  (Recordtypeira_state(v13 v12,v11,v10,v9,v8,v7,v6,v5,v4,v3,v2,v1)));
+  fun  ira_state_node_tag_fupd v13 =
+    (fn  v14 =>
+      case  v14
+      of  Recordtypeira_state(v12,v11,v10,v9,v8,v7,v6,v5,v4,v3,v2,v1) =>  (Recordtypeira_state(v12,v13 v11,v10,v9,v8,v7,v6,v5,v4,v3,v2,v1)));
+  fun  ira_state_degrees_fupd v13 =
+    (fn  v14 =>
+      case  v14
+      of  Recordtypeira_state(v12,v11,v10,v9,v8,v7,v6,v5,v4,v3,v2,v1) =>  (Recordtypeira_state(v12,v11,v13 v10,v9,v8,v7,v6,v5,v4,v3,v2,v1)));
+  fun  ira_state_dim_fupd v13 =
+    (fn  v14 =>
+      case  v14
+      of  Recordtypeira_state(v12,v11,v10,v9,v8,v7,v6,v5,v4,v3,v2,v1) =>  (Recordtypeira_state(v12,v11,v10,v13 v9,v8,v7,v6,v5,v4,v3,v2,v1)));
+  fun  ira_state_simp_wl_fupd v13 =
+    (fn  v14 =>
+      case  v14
+      of  Recordtypeira_state(v12,v11,v10,v9,v8,v7,v6,v5,v4,v3,v2,v1) =>  (Recordtypeira_state(v12,v11,v10,v9,v13 v8,v7,v6,v5,v4,v3,v2,v1)));
+  fun  ira_state_spill_wl_fupd v13 =
+    (fn  v14 =>
+      case  v14
+      of  Recordtypeira_state(v12,v11,v10,v9,v8,v7,v6,v5,v4,v3,v2,v1) =>  (Recordtypeira_state(v12,v11,v10,v9,v8,v13 v7,v6,v5,v4,v3,v2,v1)));
+  fun  ira_state_freeze_wl_fupd v13 =
+    (fn  v14 =>
+      case  v14
+      of  Recordtypeira_state(v12,v11,v10,v9,v8,v7,v6,v5,v4,v3,v2,v1) =>  (Recordtypeira_state(v12,v11,v10,v9,v8,v7,v13 v6,v5,v4,v3,v2,v1)));
+  fun  ira_state_avail_moves_wl_fupd v13 =
+    (fn  v14 =>
+      case  v14
+      of  Recordtypeira_state(v12,v11,v10,v9,v8,v7,v6,v5,v4,v3,v2,v1) =>  (Recordtypeira_state(v12,v11,v10,v9,v8,v7,v6,v13 v5,v4,v3,v2,v1)));
+  fun  ira_state_unavail_moves_wl_fupd v13 =
+    (fn  v14 =>
+      case  v14
+      of  Recordtypeira_state(v12,v11,v10,v9,v8,v7,v6,v5,v4,v3,v2,v1) =>  (Recordtypeira_state(v12,v11,v10,v9,v8,v7,v6,v5,v13 v4,v3,v2,v1)));
+  fun  ira_state_coalesced_fupd v13 =
+    (fn  v14 =>
+      case  v14
+      of  Recordtypeira_state(v12,v11,v10,v9,v8,v7,v6,v5,v4,v3,v2,v1) =>  (Recordtypeira_state(v12,v11,v10,v9,v8,v7,v6,v5,v4,v13 v3,v2,v1)));
+  fun  ira_state_move_related_fupd v13 =
+    (fn  v14 =>
+      case  v14
+      of  Recordtypeira_state(v12,v11,v10,v9,v8,v7,v6,v5,v4,v3,v2,v1) =>  (Recordtypeira_state(v12,v11,v10,v9,v8,v7,v6,v5,v4,v3,v13 v2,v1)));
+  fun  ira_state_stack_fupd v13 =
+    (fn  v14 =>
+      case  v14
+      of  Recordtypeira_state(v12,v11,v10,v9,v8,v7,v6,v5,v4,v3,v2,v1) =>  (Recordtypeira_state(v12,v11,v10,v9,v8,v7,v6,v5,v4,v3,v2,v13 v1)));
+  datatype reg_alloc_ra_state =  Recordtypera_state of  int list list *  reg_alloc_tag list *  int list *  int *  int list *  int list *  int list *  (int *  (int *  int)) list *  (int *  (int *  int)) list *  int option list *  bool list *  int list;
+  fun  ra_state_adj_ls v13 =
+    case  v13
+    of  Recordtypera_state(v12,v11,v10,v9,v8,v7,v6,v5,v4,v3,v2,v1) =>  v12;
+  fun  ra_state_node_tag v13 =
+    case  v13
+    of  Recordtypera_state(v12,v11,v10,v9,v8,v7,v6,v5,v4,v3,v2,v1) =>  v11;
+  fun  ra_state_degrees v13 =
+    case  v13
+    of  Recordtypera_state(v12,v11,v10,v9,v8,v7,v6,v5,v4,v3,v2,v1) =>  v10;
+  fun  ra_state_dim v13 =
+    case  v13
+    of  Recordtypera_state(v12,v11,v10,v9,v8,v7,v6,v5,v4,v3,v2,v1) =>  v9;
+  fun  ra_state_simp_wl v13 =
+    case  v13
+    of  Recordtypera_state(v12,v11,v10,v9,v8,v7,v6,v5,v4,v3,v2,v1) =>  v8;
+  fun  ra_state_spill_wl v13 =
+    case  v13
+    of  Recordtypera_state(v12,v11,v10,v9,v8,v7,v6,v5,v4,v3,v2,v1) =>  v7;
+  fun  ra_state_freeze_wl v13 =
+    case  v13
+    of  Recordtypera_state(v12,v11,v10,v9,v8,v7,v6,v5,v4,v3,v2,v1) =>  v6;
+  fun  ra_state_avail_moves_wl v13 =
+    case  v13
+    of  Recordtypera_state(v12,v11,v10,v9,v8,v7,v6,v5,v4,v3,v2,v1) =>  v5;
+  fun  ra_state_unavail_moves_wl v13 =
+    case  v13
+    of  Recordtypera_state(v12,v11,v10,v9,v8,v7,v6,v5,v4,v3,v2,v1) =>  v4;
+  fun  ra_state_coalesced v13 =
+    case  v13
+    of  Recordtypera_state(v12,v11,v10,v9,v8,v7,v6,v5,v4,v3,v2,v1) =>  v3;
+  fun  ra_state_move_related v13 =
+    case  v13
+    of  Recordtypera_state(v12,v11,v10,v9,v8,v7,v6,v5,v4,v3,v2,v1) =>  v2;
+  fun  ra_state_stack v13 =
+    case  v13
+    of  Recordtypera_state(v12,v11,v10,v9,v8,v7,v6,v5,v4,v3,v2,v1) =>  v1;
+  fun  ra_state_adj_ls_fupd v13 =
+    (fn  v14 =>
+      case  v14
+      of  Recordtypera_state(v12,v11,v10,v9,v8,v7,v6,v5,v4,v3,v2,v1) =>  (Recordtypera_state(v13 v12,v11,v10,v9,v8,v7,v6,v5,v4,v3,v2,v1)));
+  fun  ra_state_node_tag_fupd v13 =
+    (fn  v14 =>
+      case  v14
+      of  Recordtypera_state(v12,v11,v10,v9,v8,v7,v6,v5,v4,v3,v2,v1) =>  (Recordtypera_state(v12,v13 v11,v10,v9,v8,v7,v6,v5,v4,v3,v2,v1)));
+  fun  ra_state_degrees_fupd v13 =
+    (fn  v14 =>
+      case  v14
+      of  Recordtypera_state(v12,v11,v10,v9,v8,v7,v6,v5,v4,v3,v2,v1) =>  (Recordtypera_state(v12,v11,v13 v10,v9,v8,v7,v6,v5,v4,v3,v2,v1)));
+  fun  ra_state_dim_fupd v13 =
+    (fn  v14 =>
+      case  v14
+      of  Recordtypera_state(v12,v11,v10,v9,v8,v7,v6,v5,v4,v3,v2,v1) =>  (Recordtypera_state(v12,v11,v10,v13 v9,v8,v7,v6,v5,v4,v3,v2,v1)));
+  fun  ra_state_simp_wl_fupd v13 =
+    (fn  v14 =>
+      case  v14
+      of  Recordtypera_state(v12,v11,v10,v9,v8,v7,v6,v5,v4,v3,v2,v1) =>  (Recordtypera_state(v12,v11,v10,v9,v13 v8,v7,v6,v5,v4,v3,v2,v1)));
+  fun  ra_state_spill_wl_fupd v13 =
+    (fn  v14 =>
+      case  v14
+      of  Recordtypera_state(v12,v11,v10,v9,v8,v7,v6,v5,v4,v3,v2,v1) =>  (Recordtypera_state(v12,v11,v10,v9,v8,v13 v7,v6,v5,v4,v3,v2,v1)));
+  fun  ra_state_freeze_wl_fupd v13 =
+    (fn  v14 =>
+      case  v14
+      of  Recordtypera_state(v12,v11,v10,v9,v8,v7,v6,v5,v4,v3,v2,v1) =>  (Recordtypera_state(v12,v11,v10,v9,v8,v7,v13 v6,v5,v4,v3,v2,v1)));
+  fun  ra_state_avail_moves_wl_fupd v13 =
+    (fn  v14 =>
+      case  v14
+      of  Recordtypera_state(v12,v11,v10,v9,v8,v7,v6,v5,v4,v3,v2,v1) =>  (Recordtypera_state(v12,v11,v10,v9,v8,v7,v6,v13 v5,v4,v3,v2,v1)));
+  fun  ra_state_unavail_moves_wl_fupd v13 =
+    (fn  v14 =>
+      case  v14
+      of  Recordtypera_state(v12,v11,v10,v9,v8,v7,v6,v5,v4,v3,v2,v1) =>  (Recordtypera_state(v12,v11,v10,v9,v8,v7,v6,v5,v13 v4,v3,v2,v1)));
+  fun  ra_state_coalesced_fupd v13 =
+    (fn  v14 =>
+      case  v14
+      of  Recordtypera_state(v12,v11,v10,v9,v8,v7,v6,v5,v4,v3,v2,v1) =>  (Recordtypera_state(v12,v11,v10,v9,v8,v7,v6,v5,v4,v13 v3,v2,v1)));
+  fun  ra_state_move_related_fupd v13 =
+    (fn  v14 =>
+      case  v14
+      of  Recordtypera_state(v12,v11,v10,v9,v8,v7,v6,v5,v4,v3,v2,v1) =>  (Recordtypera_state(v12,v11,v10,v9,v8,v7,v6,v5,v4,v3,v13 v2,v1)));
+  fun  ra_state_stack_fupd v13 =
+    (fn  v14 =>
+      case  v14
+      of  Recordtypera_state(v12,v11,v10,v9,v8,v7,v6,v5,v4,v3,v2,v1) =>  (Recordtypera_state(v12,v11,v10,v9,v8,v7,v6,v5,v4,v3,v2,v13 v1)));
   datatype ( 'a  ,  'b ) ml_monadBase_exc =  Failure of  'b
-                                           |  Success of  'a ;
-  fun  reg_alloc_aux k =
-    (fn  mtable =>
-      (fn  ct =>
-        (fn  forced =>
-          (fn  x =>
-            let val  degrees = Array.array ( (snd (snd x)), 0)
-                val  node_tag = Array.array ( (snd (snd x)), Atemp)
-                val  adj_ls = Array.array ( (snd (snd x)), [] )
-                val  stack = ref( [] )
-                val  spill_wl = ref( [] )
-                val  simp_wl = ref( [] )
-                val  dim = ref( (snd (snd x)))
-                fun  st_ex_foreach v5 v4 =
-                    case  v5
-                    of  []  =>  ()
-                    |   v3::v2 =>  (let val  v1 = v4 v3
-                                     in
-                                      st_ex_foreach v2 v4
-                                     end)
-                fun  st_ex_map v5 v6 =
-                    case  v6
-                    of  []  =>  []
-                     |   v4::v3 =>  (let val  v2 = v5 v4
-                                         val  v1 = st_ex_map v5 v3
-                                      in
-                                       v2::v1
-                                      end)
-                fun  st_ex_partition v4 v6 v7 v5 =
-                    case  v6
-                    of  []  =>  (v7,v5)
-                    |   v3::v2 =>  (let val  v1 = v4 v3
-                                     in
-                                      if  v1
-                                       then  (st_ex_partition v4 v2 (v3::v7) v5)
-                                      else  (st_ex_partition v4 v2 v7 (v3::v5))
-                                    end)
-                fun  st_ex_filter v4 v6 v5 =
-                    case  v6
-                    of  []  =>  v5
-                    |   v3::v2 =>  (let val  v1 = v4 v3
-                                     in
-                                      if  v1
-                                       then  (st_ex_filter v4 v2 (v3::v5))
-                                      else  (st_ex_filter v4 v2 v5)
-                                    end)
-                val  dec_deg =
-              (fn  v2 =>
-                let val  v1 =
-                  (Array.sub ( degrees, v2))
-                  handle  Subscript =>  raise  let val  x = ()
-                                              in
-                                                Readerror(x)
-                                              end
+   |  Success of  'a ;
+  fun  reg_alloc_aux alg =
+    (fn  sc =>
+      (fn  k =>
+        (fn  mtable =>
+          (fn  ct =>
+            (fn  forced =>
+              (fn  x =>
+                let val  move_related = Array.array ( (snd (snd x)),(0 < 0))
+                    val  coalesced = Array.array ( (snd (snd x)),NONE)
+                    val  degrees = Array.array ( (snd (snd x)),0)
+                    val  node_tag = Array.array ( (snd (snd x)),Atemp)
+                    val  adj_ls = Array.array ( (snd (snd x)),[] )
+                    val  stack = ref([] )
+                    val  unavail_moves_wl = ref([] )
+                    val  avail_moves_wl = ref([] )
+                    val  freeze_wl = ref([] )
+                    val  spill_wl = ref([] )
+                    val  simp_wl = ref([] )
+                    val  dim = ref((snd (snd x)))
+                    fun  st_ex_foreach v5 v4 =
+                case  v5
+                of  []  =>  ()
+                |   v3::v2 =>  (let val  v1 = v4 v3
                  in
-                  (Array.update ( degrees, v2, (v1 - 1)))
-                  handle  Subscript =>  raise  let val  x = ()
-                                              in
-                                                Writeerror(x)
-                                              end
+                  st_ex_foreach v2 v4
                  end)
-                val  dec_degree =
-              (fn  v3 =>
-                let val  v2 = !( dim)
-                in
-                  if  (v3 < v2)
-                  then  (let val  v1 =
-                           (Array.sub ( adj_ls, v3))
-                           handle  Subscript =>  raise  let val  x = ()
-                                                       in
-                                                         Readerror(x)
-                                                       end
-                          in
-                           st_ex_foreach v1 dec_deg
-                          end)
-                  else  ()
-                end)
-                val  add_simp_wl =
-              (fn  v2 =>
-                let val  v1 = !( simp_wl)
-                in
-                  simp_wl := (append v2 v1)
-                end)
-                val  add_stack =
-              (fn  v2 =>
-                let val  v1 = !( stack)
-                in
-                  stack := (append v2 v1)
-                end)
-                val  split_degree =
-              (fn  v2 =>
-                (fn  v3 =>
-                  (fn  v4 =>
-                    if  (v4 < v2)
-                    then  (let val  v1 =
-                             (Array.sub ( degrees, v4))
-                             handle  Subscript =>  raise  let val  x = ()
-                                                         in
-                                                           Readerror(x)
-                                                         end
-                            in
-                             v1 < v3
-                            end)
-                    else  (0 <= 0))))
-                val  unspill =
-              (fn  v7 =>
-                let val  v6 = !( dim)
-                    val  v5 = !( spill_wl)
-                    val  v4 =
-                  st_ex_partition (split_degree v6 v7) v5 [] []
+                    fun  st_ex_map v5 v6 =
+                case  v6
+                of  []  =>  []
+                 |   v4::v3 =>  (let val  v2 = v5 v4
+                    val  v1 = st_ex_map v5 v3
                  in
-                  case  v4
-                  of  (v3,v2) =>  (let val  v1 = spill_wl := v2
-                                    in
-                                     add_simp_wl v3
-                                    end)
-                end)
-                val  do_simplify =
-              (fn  v6 =>
-                let val  v5 = !( simp_wl)
-                in
-                  if  (null v5)
-                  then  (0 < 0)
-                  else  (let val  v4 = st_ex_foreach v5 dec_degree
-                             val  v3 = add_stack v5
-                             val  v2 = simp_wl := []
-                              val  v1 = unspill v6
-                          in
-                           0 <= 0
-                          end)
-                end)
-                fun  st_ex_list_max_deg v7 v5 v6 v8 v4 =
-                    case  v7
-                    of  []  =>  (v6,v4)
-                    |   v3::v2 =>  (if  (v3 < v5)
-                                    then  (let val  v1 =
-                                             (Array.sub ( degrees, v3))
-                                             handle  Subscript =>  raise  let val  x =
-                                                                           ()
-                                                                         in
-                                                                           Readerror(x)
-                                                                         end
-                                            in
-                                             if  (v8 < v1)
-                                             then  (st_ex_list_max_deg v2 v5 v3 v1 (v6::v4))
-                                             else  (st_ex_list_max_deg v2 v5 v6 v8 (v3::v4))
-                                           end)
-                                    else  (st_ex_list_max_deg v2 v5 v6 v8 v4))
-                val  do_spill =
-              (fn  v13 =>
-                let val  v12 = !( spill_wl)
-                    val  v11 = !( dim)
-                in
-                  case  v12
-                  of  []  =>  (0 < 0)
-                  |   v10::v9 =>  (if  (v10 >= v11)
-                                   then  (0 <= 0)
-                                   else  (let val  v8 =
-                                            (Array.sub ( degrees, v10))
-                                            handle  Subscript =>  raise  let val  x =
-                                                                          ()
-                                                                        in
-                                                                          Readerror(x)
-                                                                        end
-                                              val  v7 =
-                                            st_ex_list_max_deg v9 v11 v10 v8 []
-                                           in
-                                            case  v7
-                                            of  (v6,v5) =>  (let val  v4 =
-                                                               dec_deg v6
-                                                                 val  v3 =
-                                                               unspill v13
-                                                                 val  v2 =
-                                                               add_stack [v6]
-                                                                 val  v1 =
-                                                               spill_wl := v5
-                                                              in
-                                                               0 <= 0
-                                                              end)
-                                          end))
-                end)
-                val  do_step =
-              (fn  v3 =>
-                let val  v2 = do_simplify v3
+                  v2::v1
+                 end)
+                    fun  st_ex_partition v4 v6 v7 v5 =
+                case  v6
+                of  []  =>  (v7,v5)
+                |   v3::v2 =>  (let val  v1 = v4 v3
                  in
-                  if  v2
-                   then  ()
-                  else  (let val  v1 = do_spill v3
-                          in
-                           ()
-                         end)
+                  if  v1
+                 then  (st_ex_partition v4 v2 (v3::v7) v5)
+                else  (st_ex_partition v4 v2 v7 (v3::v5))
                 end)
-                fun  rpt_do_step v2 v3 =
-                    if  (v3 = 0)
-                    then  ()
-                    else  (let val  v1 = do_step v2
-                            in
-                             rpt_do_step v2 (let val  k = v3 - 1
-                                              in
-                                               if  (k < 0)
-                                               then  0
-                                                else  k
-                                              end)
-                           end)
-                fun  remove_colours v10 v9 =
-                    case  v9
-                    of  []  =>  []
-                     |   v8::v7 =>  (case  v10
-                                     of  []  =>  (v8::v7)
-                                     |   (v6::v5) =>  (let val  v4 =
-                                                         (Array.sub ( node_tag, v6))
-                                                         handle  Subscript =>  raise  let val  x =
-                                                                                       ()
-                                                                                     in
-                                                                                       Readerror(x)
-                                                                                     end
-                                                           val  v3 =
-                                                         case  v4
-                                                         of  Fixed(v2) =>  (remove_colours v5 (filter (fn  v1 =>
-                                                                                                        ((v1 = v2) = (0 < 0))) (v8::v7)))
-                                                         |   Atemp =>  (remove_colours v5 (v8::v7))
-                                                         |   Stemp =>  (remove_colours v5 (v8::v7))
-                                                       in
-                                                         v3
-                                                        end))
-                val  assign_atemp_tag =
-              (fn  v11 =>
-                (fn  v10 =>
-                  (fn  v9 =>
-                    let val  v8 =
-                      (Array.sub ( node_tag, v9))
-                      handle  Subscript =>  raise  let val  x = ()
-                                                  in
-                                                    Readerror(x)
-                                                  end
-                     in
-                      case  v8
-                      of  Fixed(v1) =>  ()
-                      |   Atemp =>  (let val  v7 =
-                                       (Array.sub ( adj_ls, v9))
-                                       handle  Subscript =>  raise  let val  x =
-                                                                     ()
-                                                                   in
-                                                                     Readerror(x)
-                                                                   end
-                                         val  v6 = remove_colours v7 v11
-                                      in
-                                       case  v6
-                                       of  []  =>  ((Array.update ( node_tag, v9, Stemp))
-                                                    handle  Subscript =>  raise  let val  x =
-                                                                                  ()
-                                                                                in
-                                                                                  Writeerror(x)
-                                                                                end)
-                                       |   v5::v4 =>  (let val  v3 =
-                                                         v10 v9 v6
-                                                        in
-                                                         case  v3
-                                                         of  NONE =>  ((Array.update ( node_tag, v9, (Fixed(v5))))
-                                                                       handle  Subscript =>  raise  let val  x =
-                                                                                                     ()
-                                                                                                   in
-                                                                                                     Writeerror(x)
-                                                                                                   end)
-                                                         |   SOME(v2) =>  ((Array.update ( node_tag, v9, (Fixed(v2))))
-                                                                           handle  Subscript =>  raise  let val  x =
-                                                                                                         ()
-                                                                                                       in
-                                                                                                         Writeerror(x)
-                                                                                                       end)
-                                                       end)
-                                     end)
-                      |   Stemp =>  ()
-                    end)))
-                val  assign_atemps =
-              (fn  v11 =>
-                (fn  v9 =>
-                  (fn  v10 =>
-                    let val  v8 = !( dim)
-                        val  v7 = filter (fn  v1 => (v1 < v8)) v9
-                        val  v6 = genlist (fn  v2 => v2) v11
-                        val  v5 = genlist (fn  v3 => v3) v8
-                        val  v4 =
-                      st_ex_foreach v7 (assign_atemp_tag v6 v10)
+                    fun  st_ex_filter v4 v6 v5 =
+                case  v6
+                of  []  =>  v5
+                |   v3::v2 =>  (let val  v1 = v4 v3
+                 in
+                  if  v1
+                 then  (st_ex_filter v4 v2 (v3::v5))
+                else  (st_ex_filter v4 v2 v5)
+                end)
+                    val  dec_deg =
+                  (fn  v2 =>
+                    let val  v1 = Array.sub ( degrees,v2)
                     in
-                      st_ex_foreach v5 (assign_atemp_tag v6 v10)
-                    end)))
-                val  assign_stemp_tag =
-              (fn  v10 =>
-                (fn  v9 =>
-                  let val  v8 =
-                    (Array.sub ( node_tag, v9))
-                    handle  Subscript =>  raise  let val  x = ()
-                                                in
-                                                  Readerror(x)
-                                                end
-                   in
-                    case  v8
-                    of  Fixed(v1) =>  ()
-                    |   Atemp =>  ()
-                    |   Stemp =>  (let val  v7 =
-                                     (Array.sub ( adj_ls, v9))
-                                     handle  Subscript =>  raise  let val  x =
-                                                                   ()
-                                                                 in
-                                                                   Readerror(x)
-                                                                 end
-                                       val  v6 =
-                                     st_ex_map (fn  v2 =>
-                                                 ((Array.sub ( node_tag, v2))
-                                                  handle  Subscript =>  raise  let val  x =
-                                                                                ()
-                                                                              in
-                                                                                Readerror(x)
-                                                                              end)) v7
-                                       val  v5 =
-                                     unbound_colour v10 (qsort (fn  v4 =>
-                                                                 (fn  v3 =>
-                                                                   (v4 <= v3))) (map tag_col v6))
-                                   in
-                                     (Array.update ( node_tag, v9, (Fixed(v5))))
-                                     handle  Subscript =>  raise  let val  x =
-                                                                   ()
-                                                                 in
-                                                                   Writeerror(x)
-                                                                 end
-                                    end)
-                  end))
-                val  assign_stemps =
-              (fn  v4 =>
-                let val  v3 = !( dim)
-                    val  v2 = genlist (fn  v1 => v1) v3
-                 in
-                  st_ex_foreach v2 (assign_stemp_tag v4)
-                end)
-                fun  first_match_col v5 v6 =
-                    case  v6
-                    of  []  =>  NONE
-                    |   v4::v3 =>  (let val  v2 =
-                                      (Array.sub ( node_tag, v4))
-                                      handle  Subscript =>  raise  let val  x =
-                                                                    ()
-                                                                  in
-                                                                    Readerror(x)
-                                                                  end
-                                     in
-                                      case  v2
-                                      of  Fixed(v1) =>  (if  (member v1 v5)
-                                                         then  (SOME(v1))
-                                                         else  (first_match_col v5 v3))
-                                      |   Atemp =>  (first_match_col v5 v3)
-                                      |   Stemp =>  (first_match_col v5 v3)
-                                    end)
-                val  biased_pref =
-              (fn  v4 =>
-                (fn  v5 =>
+                      Array.update ( degrees, v2,(let val  k = v1 - 1
+                     in
+                      if  (k < 0)
+                    then  0
+                     else  k
+                     end))
+                    end)
+                    val  dec_degree =
                   (fn  v3 =>
-                    case  (lookup v5 v4)
-                    of  NONE =>  NONE
-                    |   SOME(v2) =>  ((first_match_col v3 v2)
-                                      handle  Readerror(v1) =>  NONE))))
-                val  insert_edge =
-              (fn  v4 =>
-                (fn  v5 =>
-                  let val  v3 =
-                    (Array.sub ( adj_ls, v4))
-                    handle  Subscript =>  raise  let val  x = ()
-                                                in
-                                                  Readerror(x)
-                                                end
-                      val  v2 =
-                    (Array.sub ( adj_ls, v5))
-                    handle  Subscript =>  raise  let val  x = ()
-                                                in
-                                                  Readerror(x)
-                                                end
-                   in
-                    if  (member v5 v3)
-                    then  ()
-                    else  (let val  v1 =
-                             (Array.update ( adj_ls, v4, (v5::v3)))
-                             handle  Subscript =>  raise  let val  x = ()
-                                                         in
-                                                           Writeerror(x)
-                                                         end
-                            in
-                             (Array.update ( adj_ls, v5, (v4::v2)))
-                             handle  Subscript =>  raise  let val  x = ()
-                                                         in
-                                                           Writeerror(x)
-                                                         end
-                            end)
-                  end))
-                fun  list_insert_edge v5 v4 =
-                    case  v4
-                    of  []  =>  ()
-                    |   v3::v2 =>  (let val  v1 = insert_edge v5 v3
-                                     in
-                                      list_insert_edge v5 v2
-                                     end)
-                fun  clique_insert_edge v4 =
-                    case  v4
-                    of  []  =>  ()
-                    |   v3::v2 =>  (let val  v1 = list_insert_edge v3 v2
-                                     in
-                                      clique_insert_edge v2
-                                     end)
-                fun  extend_clique v5 v4 =
-                    case  v5
-                    of  []  =>  v4
-                    |   v3::v2 =>  (if  (member v3 v4)
-                                    then  (extend_clique v2 v4)
-                                    else  (let val  v1 =
-                                             list_insert_edge v3 v4
-                                            in
-                                             extend_clique v2 (v3::v4)
-                                           end))
-                fun  mk_graph v26 v25 v24 =
-                    case  v25
-                    of  Delta(v8,v7) =>  (let val  v6 = map v26 v8
-                                              val  v5 = map v26 v7
-                                              val  v4 =
-                                            extend_clique v6 v24
-                                              val  v3 =
-                                            filter (fn  v1 =>
-                                                     ((member v1 v6) = (0 < 0))) v4
-                                              val  v2 =
-                                            extend_clique v5 v3
-                                           in
-                                            v2
-                                           end)
-                    |   Set(v11) =>  (let val  v10 =
-                                        map v26 (map fst (toalist v11))
-                                          val  v9 = clique_insert_edge v10
-                                       in
-                                        v10
-                                       end)
-                    |   Branch(v20,v19,v18) =>  (let val  v17 =
-                                                   mk_graph v26 v19 v24
-                                                     val  v16 =
-                                                   mk_graph v26 v18 v24
-                                                  in
-                                                   case  v20
-                                                   of  NONE =>  (let val  v12 =
-                                                                   extend_clique v17 v16
-                                                                  in
-                                                                   v12
-                                                                  end)
-                                                   |   SOME(v15) =>  (let val  v14 =
-                                                                        map v26 (map fst (toalist v15))
-                                                                          val  v13 =
-                                                                        clique_insert_edge v14
-                                                                       in
-                                                                        v14
-                                                                       end)
-                                                 end)
-                    |   Seq(v23,v22) =>  (let val  v21 =
-                                            mk_graph v26 v22 v24
-                                           in
-                                            mk_graph v26 v23 v21
-                                           end)
-                fun  extend_graph v6 v7 =
-                    case  v7
-                    of  []  =>  ()
-                    |   v5::v4 =>  (case  v5
-                                    of  (v3,v2) =>  (let val  v1 =
-                                                       insert_edge (v6 v3) (v6 v2)
-                                                     in
-                                                       extend_graph v6 v4
-                                                      end))
-                val  mk_tags =
-              (fn  v7 =>
-                (fn  v6 =>
-                  let val  v5 = genlist (fn  v1 => v1) v7
-                   in
-                    st_ex_foreach v5 (fn  v4 =>
-                                       (let val  v3 = v6 v4
-                                            val  v2 = v3 mod 4
-                                         in
-                                          if  (v2 = 1)
-                                          then  ((Array.update ( node_tag, v4, Atemp))
-                                                 handle  Subscript =>  raise  let val  x =
-                                                                               ()
-                                                                             in
-                                                                               Writeerror(x)
-                                                                             end)
-                                          else  (if  (v2 = 3)
-                                                 then  ((Array.update ( node_tag, v4, Stemp))
-                                                        handle  Subscript =>  raise  let val  x =
-                                                                                      ()
-                                                                                    in
-                                                                                      Writeerror(x)
-                                                                                    end)
-                                                 else  ((Array.update ( node_tag, v4, (Fixed(v3 div 2))))
-                                                        handle  Subscript =>  raise  let val  x =
-                                                                                      ()
-                                                                                    in
-                                                                                      Writeerror(x)
-                                                                                    end))
-                                        end))
-                  end))
-                val  init_ra_state =
-              (fn  v11 =>
-                (fn  v9 =>
-                  (fn  v10 =>
-                    case  (v9,v10)
-                    of  (v8,v7) =>  (case  v7
-                                     of  (v6,v5) =>  (case  v5
-                                                      of  (v4,v3) =>  (let val  v2 =
-                                                                         mk_graph (sp_default v6) v11 []
-                                                                            val  v1 =
-                                                                         extend_graph (sp_default v6) v8
-                                                                        in
-                                                                         mk_tags v3 (sp_default v4)
-                                                                       end))))))
-                val  is_atemp =
-              (fn  v2 =>
-                let val  v1 =
-                  (Array.sub ( node_tag, v2))
-                  handle  Subscript =>  raise  let val  x = ()
-                                              in
-                                                Readerror(x)
-                                              end
+                    let val  v2 = !(dim)
+                    in
+                      if  (v3 < v2)
+                    then  (let val  v1 = Array.sub ( adj_ls,v3)
+                    in
+                      st_ex_foreach v1 dec_deg
+                     end)
+                    else  ()
+                    end)
+                    val  add_simp_wl =
+                  (fn  v2 =>
+                    let val  v1 = !(simp_wl)
+                    in
+                      simp_wl := (v2 @ v1)
+                    end)
+                    val  add_freeze_wl =
+                  (fn  v2 =>
+                    let val  v1 = !(freeze_wl)
+                    in
+                      freeze_wl := (v2 @ v1)
+                    end)
+                    val  push_stack =
+                  (fn  v4 =>
+                    let val  v3 = !(stack)
+                        val  v2 = Array.update ( degrees, v4,0)
+                        val  v1 = Array.update ( move_related, v4,(0 < 0))
+                    in
+                      stack := (v4::v3)
+                    end)
+                    val  add_unavail_moves_wl =
+                  (fn  v2 =>
+                    let val  v1 = !(unavail_moves_wl)
+                    in
+                      unavail_moves_wl := (v2 @ v1)
+                    end)
+                    val  split_degree =
+                  (fn  v2 =>
+                    (fn  v3 =>
+                      (fn  v4 =>
+                        if  (v4 < v2)
+                        then  (let val  v1 = Array.sub ( degrees,v4)
+                        in
+                          v1 < v3
+                         end)
+                        else  (0 <= 0))))
+                    val  revive_moves =
+                  (fn  v16 =>
+                    let val  v15 =
+                      st_ex_map (fn  v1 => (Array.sub ( adj_ls,v1))) v16
+                        val  v14 = !(unavail_moves_wl)
+                        val  v13 = !(avail_moves_wl)
+                        val  v12 = List.concat v15
+                        val  v6 =
+                      partition (fn  v11 =>
+                        (case  v11
+                        of  (v10,v9) =>  (case  v9
+                        of  (v8,v7) =>  ((member v8 v12) orelse  (member v7 v12))))) v14
+                     in
+                      case  v6
+                    of  (v5,v4) =>  (let val  v3 = smerge (sort_moves v5) v13
+                        val  v2 = avail_moves_wl := v3
+                     in
+                      unavail_moves_wl := v4
+                     end)
+                    end)
+                    val  unspill =
+                  (fn  v13 =>
+                    let val  v12 = !(dim)
+                        val  v11 = !(spill_wl)
+                        val  v10 =
+                      st_ex_partition (split_degree v12 v13) v11 [] []
+                     in
+                      case  v10
+                    of  (v9,v8) =>  (let val  v7 = revive_moves v9
+                        val  v6 =
+                      st_ex_partition (fn  v1 =>
+                        (Array.sub ( move_related,v1))) v9 [] []
+                     in
+                      case  v6
+                    of  (v5,v4) =>  (let val  v3 = spill_wl := v8
+                        val  v2 = add_simp_wl v4
+                     in
+                      add_freeze_wl v5
+                     end)
+                    end)
+                    end)
+                    val  do_simplify =
+                  (fn  v6 =>
+                    let val  v5 = !(simp_wl)
+                    in
+                      if  (List.null v5)
+                    then  (0 < 0)
+                    else  (let val  v4 = st_ex_foreach v5 dec_degree
+                        val  v3 = st_ex_foreach v5 push_stack
+                        val  v2 = simp_wl := []
+                         val  v1 = unspill v6
+                     in
+                      0 <= 0
+                     end)
+                    end)
+                    val  inc_deg =
+                  (fn  v3 =>
+                    (fn  v2 =>
+                      let val  v1 = Array.sub ( degrees,v3)
+                      in
+                        Array.update ( degrees, v3,(v1 + v2))
+                      end))
+                    val  insert_edge =
+                  (fn  v4 =>
+                    (fn  v5 =>
+                      let val  v3 = Array.sub ( adj_ls,v4)
+                          val  v2 = Array.sub ( adj_ls,v5)
+                      in
+                        if  (member v5 v3)
+                      then  ()
+                      else  (let val  v1 = Array.update ( adj_ls, v4,(v5::v3))
+                      in
+                        Array.update ( adj_ls, v5,(v4::v2))
+                      end)
+                      end))
+                    fun  list_insert_edge v5 v4 =
+                case  v4
+                of  []  =>  ()
+                |   v3::v2 =>  (let val  v1 = insert_edge v5 v3
                  in
-                  v1 = Atemp
+                  list_insert_edge v5 v2
                  end)
-                val  init_alloc1_heu =
-              (fn  v12 =>
-                (fn  v13 =>
-                  let val  v11 = genlist (fn  v1 => v1) v12
-                      val  v10 =
-                    st_ex_foreach v11 (fn  v3 =>
-                                        (let val  v2 =
-                                           (Array.sub ( adj_ls, v3))
-                                           handle  Subscript =>  raise  let val  x =
-                                                                         ()
-                                                                       in
-                                                                         Readerror(x)
-                                                                       end
-                                          in
-                                           (Array.update ( degrees, v3, (length v2)))
-                                           handle  Subscript =>  raise  let val  x =
-                                                                         ()
-                                                                       in
-                                                                         Writeerror(x)
-                                                                       end
-                                          end))
-                      val  v9 = st_ex_filter is_atemp v11 []
-                       val  v8 =
-                    st_ex_partition (split_degree v12 v13) v9 [] []
-                   in
-                    case  v8
-                    of  (v7,v6) =>  (let val  v5 = simp_wl := v7
-                                         val  v4 = spill_wl := v6
-                                      in
-                                       length v9
-                                      end)
-                  end))
-                val  do_alloc1 =
-              (fn  v5 =>
-                let val  v4 = !( dim)
-                    val  v3 = init_alloc1_heu v4 v5
-                    val  v2 = rpt_do_step v5 v3
-                    val  v1 = !( stack)
+                    val  do_coalesce_real =
+                  (fn  v15 =>
+                    (fn  v16 =>
+                      let val  v14 = Array.update ( coalesced, v16,(SOME(v15)))
+                          val  v13 = !(avail_moves_wl)
+                          val  v12 =
+                        avail_moves_wl := (List.map (pair_rename v15 v16) v13)
+                          val  v11 = !(unavail_moves_wl)
+                          val  v10 =
+                        unavail_moves_wl := (List.map (pair_rename v15 v16) v11)
+                          val  v9 = Array.sub ( adj_ls,v15)
+                          val  v8 = Array.sub ( adj_ls,v16)
+                          val  v6 =
+                        partition (fn  v7 => (member v7 v9)) v8
+                       in
+                        case  v6
+                      of  (v5,v4) =>  (let val  v3 =
+                        inc_deg v15 (List.length v4)
+                          val  v2 = list_insert_edge v15 v4
+                          val  v1 = st_ex_foreach v5 dec_deg
+                       in
+                        push_stack v16
+                       end)
+                      end))
+                    val  bg_ok =
+                  (fn  v21 =>
+                    (fn  v22 =>
+                      (fn  v23 =>
+                        let val  v20 = Array.sub ( adj_ls,v22)
+                            val  v19 = Array.sub ( adj_ls,v23)
+                            val  v17 =
+                          partition (fn  v18 => (member v18 v20)) v19
+                         in
+                          case  v17
+                        of  (v16,v15) =>  (let val  v14 =
+                          st_ex_map (fn  v1 => (Array.sub ( degrees,v1))) v15
+                            val  v12 =
+                          List.length (List.filter (fn  v13 => (v13 >= v21)) v14)
+                        in
+                          if  (v12 = 0)
+                        then  (0 <= 0)
+                        else  (let val  v10 =
+                          List.filter (fn  v11 =>
+                            ((member v11 v19) = (0 < 0))) v20
+                            val  v9 =
+                          st_ex_map (fn  v2 => (Array.sub ( degrees,v2))) v16
+                            val  v8 =
+                          st_ex_map (fn  v3 => (Array.sub ( degrees,v3))) v10
+                            val  v7 =
+                          List.length (List.filter (fn  v4 =>
+                            ((let val  k = v4 - 1
+                             in
+                              if  (k < 0)
+                            then  0
+                             else  k
+                             end) >= v21)) v9)
+                            val  v6 =
+                          List.length (List.filter (fn  v5 => (v5 >= v21)) v8)
+                        in
+                          ((v7 + v12) + v6) < v21
+                         end)
+                        end)
+                        end)))
+                    val  is_fixed =
+                  (fn  v3 =>
+                    let val  v2 = Array.sub ( node_tag,v3)
+                    in
+                      case  v2
+                    of  Fixed(v1) =>  (0 <= 0)
+                    |   Atemp =>  (0 < 0)
+                    |   Stemp =>  (0 < 0)
+                    end)
+                    val  consistency_ok =
+                  (fn  v6 =>
+                    (fn  v7 =>
+                      if  (v6 = v7)
+                      then  (0 < 0)
+                      else  (let val  v5 = !(dim)
+                      in
+                        if  ((v6 >= v5) orelse  (v7 >= v5))
+                      then  (0 < 0)
+                      else  (let val  v4 = Array.sub ( adj_ls,v7)
+                      in
+                        if  (member v6 v4)
+                      then  (0 < 0)
+                      else  (let val  v3 = is_fixed v6
+                          val  v2 = Array.sub ( move_related,v6)
+                          val  v1 = Array.sub ( move_related,v7)
+                      in
+                        (v3 orelse  v2) andalso  v1
+                       end)
+                      end)
+                      end)))
+                    fun  st_ex_first v10 v11 v12 v13 =
+                case  v12
+                of  []  =>  (NONE,v13)
+                |   v9::v8 =>  (let val  v7 = v9
+                 in
+                  case  v7
+                of  (v6,v5) =>  (case  v5
+                of  (v4,v3) =>  (let val  v2 = v10 v4 v3
+                 in
+                  if  (v2 = (0 < 0))
+                then  (st_ex_first v10 v11 v8 v13)
+                else  (let val  v1 = v11 v4 v3
+                 in
+                  if  v1
+                 then  (let val  x = ((v4,v3),v8)
                 in
-                  v1
-                 end)
-                val  extract_color =
-              (fn  v7 =>
-                let val  v6 = toalist v7
-                    val  v5 =
-                  st_ex_map (fn  v4 =>
-                              (case  v4
-                               of  (v3,v2) =>  (let val  v1 =
-                                                  (Array.sub ( node_tag, v2))
-                                                  handle  Subscript =>  raise  let val  x =
-                                                                                ()
-                                                                              in
-                                                                                Readerror(x)
-                                                                              end
-                                                 in
-                                                  (v3,extract_tag v1)
-                                                end))) v6
+                  SOME(x)
+                end,v13)
+                else  (st_ex_first v10 v11 v8 (v9::v13))
+                end)
+                end))
+                end)
+                    val  do_coalesce =
+                  (fn  v15 =>
+                    let val  v14 = !(avail_moves_wl)
+                        val  v13 =
+                      st_ex_first consistency_ok (bg_ok v15) v14 []
+                     in
+                      case  v13
+                    of  (v12,v11) =>  (let val  v10 = add_unavail_moves_wl v11
+                     in
+                      case  v12
+                    of  NONE =>  (let val  v1 = avail_moves_wl := []
+                     in
+                      0 < 0
+                     end)
+                    |   SOME(v9) =>  (case  v9
+                    of  (v8,v7) =>  (case  v8
+                    of  (v6,v5) =>  (let val  v4 = avail_moves_wl := v7
+                        val  v3 = do_coalesce_real v6 v5
+                        val  v2 = unspill v15
+                     in
+                      0 <= 0
+                     end)))
+                    end)
+                    end)
+                    val  is_not_coalesced =
+                  (fn  v2 =>
+                    let val  v1 = Array.sub ( coalesced,v2)
+                    in
+                      v1 = NONE
+                     end)
+                    val  reset_move_related =
+                  (fn  v10 =>
+                    let val  v9 = !(dim)
+                        val  v8 =
+                      st_ex_foreach (count_list v9) (fn  v1 =>
+                        (Array.update ( move_related, v1,(0 < 0))))
+                    in
+                      st_ex_foreach v10 (fn  v7 =>
+                      (case  v7
+                      of  (v6,v5) =>  (case  v5
+                      of  (v4,v3) =>  (let val  v2 =
+                        Array.update ( move_related, v4,(0 <= 0))
+                      in
+                        Array.update ( move_related, v3,(0 <= 0))
+                      end))))
+                    end)
+                    val  do_prefreeze =
+                  (fn  v21 =>
+                    let val  v20 = !(freeze_wl)
+                        val  v19 = st_ex_filter is_not_coalesced v20 []
+                         val  v18 = !(spill_wl)
+                        val  v17 = st_ex_filter is_not_coalesced v18 []
+                         val  v16 = spill_wl := v17
+                        val  v15 = !(unavail_moves_wl)
+                        val  v14 =
+                      st_ex_filter (fn  v5 =>
+                        (case  v5
+                        of  (v4,v3) =>  (case  v3
+                        of  (v2,v1) =>  (consistency_ok v2 v1)))) v15 []
+                         val  v13 = reset_move_related v14
+                        val  v12 = unavail_moves_wl := v14
+                        val  v11 =
+                      st_ex_partition (fn  v6 =>
+                        (Array.sub ( move_related,v6))) v19 [] []
+                     in
+                      case  v11
+                    of  (v10,v9) =>  (let val  v8 = add_simp_wl v9
+                        val  v7 = freeze_wl := v10
+                     in
+                      do_simplify v21
+                     end)
+                    end)
+                    val  do_freeze =
+                  (fn  v8 =>
+                    let val  v7 = !(freeze_wl)
+                    in
+                      if  (List.null v7)
+                    then  (0 < 0)
+                    else  (case  v7
+                    of  []  =>  (0 < 0)
+                    |   (v6::v5) =>  (let val  v4 = dec_degree v6
+                        val  v3 = push_stack v6
+                        val  v2 = freeze_wl := v5
+                        val  v1 = unspill v8
+                     in
+                      0 <= 0
+                     end))
+                    end)
+                    fun  st_ex_list_min_cost v10 v9 v7 v8 v5 v6 =
+                case  v9
+                of  []  =>  (v8,v6)
+                |   v4::v3 =>  (if  (v4 < v7)
+                then  (let val  v2 = Array.sub ( degrees,v4)
+                    val  v1 = safe_div (lookup_any v4 v10 0) v2
                  in
-                  fromalist v5
+                  if  (v5 > v1)
+                then  (st_ex_list_min_cost v10 v3 v7 v4 v1 (v8::v6))
+                else  (st_ex_list_min_cost v10 v3 v7 v8 v5 (v4::v6))
+                end)
+                else  (st_ex_list_min_cost v10 v3 v7 v8 v5 v6))
+                    val  do_spill =
+                  (fn  v14 =>
+                    (fn  v13 =>
+                      let val  v12 = !(spill_wl)
+                          val  v11 = !(dim)
+                      in
+                        case  v12
+                      of  []  =>  (0 < 0)
+                      |   v10::v9 =>  (if  (v10 >= v11)
+                      then  (0 <= 0)
+                      else  (let val  v8 = Array.sub ( degrees,v10)
+                          val  v7 =
+                        st_ex_list_min_cost v14 v9 v11 v10 (safe_div (lookup_any v10 v14 0) v8) []
+                       in
+                        case  v7
+                      of  (v6,v5) =>  (let val  v4 = dec_deg v6
+                          val  v3 = unspill v13
+                          val  v2 = push_stack v6
+                          val  v1 = spill_wl := v5
+                       in
+                        0 <= 0
+                       end)
+                      end))
+                      end))
+                    val  do_step =
+                  (fn  v7 =>
+                    (fn  v6 =>
+                      let val  v5 = do_simplify v6
+                       in
+                        if  v5
+                       then  ()
+                      else  (let val  v4 = do_coalesce v6
+                       in
+                        if  v4
+                       then  ()
+                      else  (let val  v3 = do_prefreeze v6
+                       in
+                        if  v3
+                       then  ()
+                      else  (let val  v2 = do_freeze v6
+                       in
+                        if  v2
+                       then  ()
+                      else  (let val  v1 = do_spill v7 v6
+                       in
+                        ()
+                      end)
+                      end)
+                      end)
+                      end)
+                      end))
+                    fun  rpt_do_step v4 v2 v3 =
+                if  (v3 = 0)
+                then  ()
+                else  (let val  v1 = do_step v4 v2
+                 in
+                  rpt_do_step v4 v2 (let val  k = v3 - 1
+                 in
+                  if  (k < 0)
+                then  0
+                 else  k
                  end)
-                val  do_reg_alloc =
-              (fn  v16 =>
-                (fn  v17 =>
-                  (fn  v18 =>
-                    (fn  v19 =>
-                      (fn  v20 =>
-                        case  (v17,(v18,(v19,v20)))
-                        of  (v15,v14) =>  (case  v14
-                                           of  (v13,v12) =>  (case  v12
-                                                              of  (v11,v10) =>  (case  v10
-                                                                                 of  (v9,v8) =>  (case  v8
-                                                                                                  of  (v7,v6) =>  (let val  v5 =
-                                                                                                                     init_ra_state v13 v11 (v9,(v7,v6))
-                                                                                                                       val  v4 =
-                                                                                                                     do_alloc1 v16
-                                                                                                                       val  v3 =
-                                                                                                                     assign_atemps v16 v4 (biased_pref (resort_moves (moves_to_sp v15 Ln)))
-                                                                                                                       val  v2 =
-                                                                                                                     assign_stemps v16
-                                                                                                                       val  v1 =
-                                                                                                                     extract_color v9
-                                                                                                                    in
-                                                                                                                     v1
-                                                                                                                    end))))))))))
-            in
-              (Success(do_reg_alloc k mtable ct forced x))
-              handle  e =>  Failure(e)
-            end))));
-  fun  reg_alloc v3 =
-    (fn  v4 =>
-      (fn  v1 => (fn  v2 => reg_alloc_aux v3 v4 v1 v2 (mk_bij v1))));
+                end)
+                    fun  remove_colours v10 v9 =
+                case  v9
+                of  []  =>  []
+                 |   v8::v7 =>  (case  v10
+                of  []  =>  (v8::v7)
+                |   (v6::v5) =>  (let val  v4 = Array.sub ( node_tag,v6)
+                    val  v3 =
+                  case  v4
+                  of  Fixed(v2) =>  (remove_colours v5 (List.filter (fn  v1 =>
+                    ((v1 = v2) = (0 < 0))) (v8::v7)))
+                  |   Atemp =>  (remove_colours v5 (v8::v7))
+                  |   Stemp =>  (remove_colours v5 (v8::v7))
+                in
+                  v3
+                 end))
+                    val  assign_atemp_tag =
+                  (fn  v11 =>
+                    (fn  v10 =>
+                      (fn  v9 =>
+                        let val  v8 = Array.sub ( node_tag,v9)
+                        in
+                          case  v8
+                        of  Fixed(v1) =>  ()
+                        |   Atemp =>  (let val  v7 = Array.sub ( adj_ls,v9)
+                            val  v6 = remove_colours v7 v11
+                         in
+                          case  v6
+                        of  []  =>  (Array.update ( node_tag, v9,Stemp))
+                        |   v5::v4 =>  (let val  v3 = v10 v9 v6
+                         in
+                          case  v3
+                        of  NONE =>  (Array.update ( node_tag, v9,(Fixed(v5))))
+                        |   SOME(v2) =>  (Array.update ( node_tag, v9,(Fixed(v2))))
+                        end)
+                        end)
+                        |   Stemp =>  ()
+                        end)))
+                    val  assign_atemps =
+                  (fn  v11 =>
+                    (fn  v9 =>
+                      (fn  v10 =>
+                        let val  v8 = !(dim)
+                            val  v7 = List.filter (fn  v1 => (v1 < v8)) v9
+                            val  v6 = genlist (fn  v2 => v2) v11
+                            val  v5 = genlist (fn  v3 => v3) v8
+                            val  v4 =
+                          st_ex_foreach v7 (assign_atemp_tag v6 v10)
+                        in
+                          st_ex_foreach v5 (assign_atemp_tag v6 v10)
+                        end)))
+                    val  assign_stemp_tag =
+                  (fn  v10 =>
+                    (fn  v9 =>
+                      let val  v8 = Array.sub ( node_tag,v9)
+                      in
+                        case  v8
+                      of  Fixed(v1) =>  ()
+                      |   Atemp =>  ()
+                      |   Stemp =>  (let val  v7 = Array.sub ( adj_ls,v9)
+                          val  v6 =
+                        st_ex_map (fn  v2 => (Array.sub ( node_tag,v2))) v7
+                          val  v5 =
+                        unbound_colour v10 (qsort (fn  v4 =>
+                          (fn  v3 => (v4 <= v3))) (List.map tag_col v6))
+                      in
+                        Array.update ( node_tag, v9,(Fixed(v5)))
+                      end)
+                      end))
+                    val  assign_stemps =
+                  (fn  v4 =>
+                    let val  v3 = !(dim)
+                        val  v2 = genlist (fn  v1 => v1) v3
+                     in
+                      st_ex_foreach v2 (assign_stemp_tag v4)
+                    end)
+                    fun  first_match_col v5 v6 =
+                case  v6
+                of  []  =>  NONE
+                |   v4::v3 =>  (let val  v2 = Array.sub ( node_tag,v4)
+                in
+                  case  v2
+                of  Fixed(v1) =>  (if  (member v1 v5)
+                then  (SOME(v1))
+                else  (first_match_col v5 v3))
+                |   Atemp =>  (first_match_col v5 v3)
+                |   Stemp =>  (first_match_col v5 v3)
+                end)
+                    val  biased_pref =
+                  (fn  v6 =>
+                    (fn  v7 =>
+                      (fn  v5 =>
+                        let val  v4 = !(dim)
+                        in
+                          if  (v7 < v4)
+                        then  (let val  v3 = Array.sub ( coalesced,v7)
+                        in
+                          case  v3
+                        of  NONE =>  (case  (lookup_1 v7 v6)
+                        of  NONE =>  NONE
+                        |   (SOME(v1)) =>  ((first_match_col v5 v1)
+                        handle  Subscript =>  NONE))
+                        |   SOME(v2) =>  ((first_match_col v5 [v2])
+                        handle  Subscript =>  NONE)
+                        end)
+                        else  NONE
+                         end)))
+                    fun  clique_insert_edge v4 =
+                case  v4
+                of  []  =>  ()
+                |   v3::v2 =>  (let val  v1 = list_insert_edge v3 v2
+                 in
+                  clique_insert_edge v2
+                 end)
+                    fun  extend_clique v5 v4 =
+                case  v5
+                of  []  =>  v4
+                |   v3::v2 =>  (if  (member v3 v4)
+                then  (extend_clique v2 v4)
+                else  (let val  v1 = list_insert_edge v3 v4
+                 in
+                  extend_clique v2 (v3::v4)
+                end))
+                    fun  mk_graph v26 v25 v24 =
+                case  v25
+                of  Delta(v8,v7) =>  (let val  v6 = List.map v26 v8
+                    val  v5 = List.map v26 v7
+                    val  v4 = extend_clique v6 v24
+                    val  v3 =
+                  List.filter (fn  v1 => ((member v1 v6) = (0 < 0))) v4
+                    val  v2 = extend_clique v5 v3
+                 in
+                  v2
+                 end)
+                |   Set(v11) =>  (let val  v10 =
+                  List.map v26 (List.map fst (toalist v11))
+                    val  v9 = clique_insert_edge v10
+                 in
+                  v10
+                 end)
+                |   Branch(v20,v19,v18) =>  (let val  v17 =
+                  mk_graph v26 v19 v24
+                    val  v16 = mk_graph v26 v18 v24
+                 in
+                  case  v20
+                of  NONE =>  (let val  v12 = extend_clique v17 v16
+                 in
+                  v12
+                 end)
+                |   SOME(v15) =>  (let val  v14 =
+                  List.map v26 (List.map fst (toalist v15))
+                    val  v13 = clique_insert_edge v14
+                 in
+                  v14
+                 end)
+                end)
+                |   Seq(v23,v22) =>  (let val  v21 = mk_graph v26 v22 v24
+                 in
+                  mk_graph v26 v23 v21
+                 end)
+                    fun  extend_graph v6 v7 =
+                case  v7
+                of  []  =>  ()
+                |   v5::v4 =>  (case  v5
+                of  (v3,v2) =>  (let val  v1 = insert_edge (v6 v3) (v6 v2)
+                in
+                  extend_graph v6 v4
+                 end))
+                    val  mk_tags =
+                  (fn  v7 =>
+                    (fn  v6 =>
+                      let val  v5 = genlist (fn  v1 => v1) v7
+                       in
+                        st_ex_foreach v5 (fn  v4 =>
+                        (let val  v3 = v6 v4
+                            val  v2 = v3 mod 4
+                         in
+                          if  (v2 = 1)
+                        then  (Array.update ( node_tag, v4,Atemp))
+                        else  (if  (v2 = 3)
+                        then  (Array.update ( node_tag, v4,Stemp))
+                        else  (Array.update ( node_tag, v4,(Fixed(v3 div 2)))))
+                        end))
+                      end))
+                    val  init_ra_state =
+                  (fn  v11 =>
+                    (fn  v9 =>
+                      (fn  v10 =>
+                        case  (v9,v10)
+                        of  (v8,v7) =>  (case  v7
+                        of  (v6,v5) =>  (case  v5
+                        of  (v4,v3) =>  (let val  v2 =
+                          mk_graph (sp_default v6) v11 []
+                             val  v1 = extend_graph (sp_default v6) v8
+                         in
+                          mk_tags v3 (sp_default v4)
+                        end))))))
+                    val  is_atemp =
+                  (fn  v2 =>
+                    let val  v1 = Array.sub ( node_tag,v2)
+                    in
+                      v1 = Atemp
+                     end)
+                    val  init_alloc1_heu =
+                  (fn  v28 =>
+                    (fn  v26 =>
+                      (fn  v27 =>
+                        let val  v25 = count_list v26
+                            val  v24 =
+                          st_ex_foreach v25 (fn  v2 =>
+                            (let val  v1 = Array.sub ( adj_ls,v2)
+                            in
+                              Array.update ( degrees, v2,(List.length v1))
+                            end))
+                            val  v23 = st_ex_filter is_atemp v25 []
+                             val  v22 =
+                          st_ex_foreach v23 (fn  v3 =>
+                            (Array.update ( move_related, v3,(0 <= 0))))
+                            val  v21 =
+                          st_ex_filter (fn  v8 =>
+                            (case  v8
+                            of  (v7,v6) =>  (case  v6
+                            of  (v5,v4) =>  (consistency_ok v5 v4)))) v28 []
+                             val  v20 = avail_moves_wl := (sort_moves v21)
+                            val  v19 = reset_move_related v21
+                            val  v18 =
+                          st_ex_partition (split_degree v26 v27) v23 [] []
+                         in
+                          case  v18
+                        of  (v17,v16) =>  (let val  v15 =
+                          st_ex_partition (fn  v9 =>
+                            (Array.sub ( move_related,v9))) v17 [] []
+                         in
+                          case  v15
+                        of  (v14,v13) =>  (let val  v12 = spill_wl := v16
+                            val  v11 = simp_wl := v13
+                            val  v10 = freeze_wl := v14
+                         in
+                          List.length v23
+                         end)
+                        end)
+                        end)))
+                    val  do_alloc1 =
+                  (fn  v6 =>
+                    (fn  v7 =>
+                      (fn  v5 =>
+                        let val  v4 = !(dim)
+                            val  v3 = init_alloc1_heu v6 v4 v5
+                            val  v2 = rpt_do_step v7 v5 v3
+                            val  v1 = !(stack)
+                        in
+                          v1
+                         end)))
+                    val  extract_color =
+                  (fn  v7 =>
+                    let val  v6 = toalist v7
+                        val  v5 =
+                      st_ex_map (fn  v4 =>
+                        (case  v4
+                        of  (v3,v2) =>  (let val  v1 = Array.sub ( node_tag,v2)
+                        in
+                          (v3,extract_tag v1)
+                        end))) v6
+                     in
+                      fromalist v5
+                     end)
+                    val  do_reg_alloc =
+                  (fn  v26 =>
+                    (fn  v27 =>
+                      (fn  v28 =>
+                        (fn  v29 =>
+                          (fn  v30 =>
+                            (fn  v31 =>
+                              (fn  v32 =>
+                                case  (v27,(v28,(v29,(v30,(v31,v32)))))
+                                of  (v25,v24) =>  (case  v24
+                                of  (v23,v22) =>  (case  v22
+                                of  (v21,v20) =>  (case  v20
+                                of  (v19,v18) =>  (case  v18
+                                of  (v17,v16) =>  (case  v16
+                                of  (v15,v14) =>  (case  v14
+                                of  (v13,v12) =>  (let val  v11 =
+                                  init_ra_state v19 v17 (v15,(v13,v12))
+                                    val  v10 =
+                                  List.map (fn  v5 =>
+                                    (case  v5
+                                    of  (v4,v3) =>  (case  v3
+                                    of  (v2,v1) =>  (v4,(sp_default v15 v2,sp_default v15 v1))))) v21
+                                    val  v9 =
+                                  do_alloc1 (if  (v26 = Simple)
+                                  then  []
+                                   else  v10) v25 v23
+                                    val  v8 =
+                                  assign_atemps v23 v9 (biased_pref (resort_moves (moves_to_sp v10 Ln)))
+                                    val  v7 = assign_stemps v23
+                                    val  v6 = extract_color v15
+                                 in
+                                  v6
+                                 end))))))))))))))
+                in
+                  (Success(do_reg_alloc alg sc k mtable ct forced x))
+                handle  e =>  Failure(e)
+                end))))));
+  fun  reg_alloc v1 =
+    (fn  v6 =>
+      (fn  v4 =>
+        (fn  v5 =>
+          (fn  v2 => (fn  v3 => reg_alloc_aux v1 v6 v4 v5 v2 v3 (mk_bij v2))))));
 end
